books/projects/smtlink/verified/tibu.lisp
@@ -1,0 +1,828 @@
+;; Copyright (C) 2026, University of British Columbia
+;; Mark Greenstreet (July 30, 2026)
+;;
+;; License: A 3-clause BSD license.
+;; See the LICENSE file distributed with ACL2
+;;
+
+(in-package "SMT")
+
+(include-book "centaur/fty/top" :dir :system)
+(include-book "clause-processors/pseudo-term-fty" :dir :system)
+;(include-book "kestrel/fty/symbol-pseudoterm-alist" :dir :system)
+(include-book "misc/beta-reduce" :dir :system)
+(include-book "tools/rewrite-dollar" :dir :system)
+(include-book "tools/easy-simplify" :dir :system)
+;(include-book "ttmrg-clause-cp")
+(include-book "ttmrg-change3")
+;(include-book "type-options")
+(include-book "ttmrg-triv3")
+(include-book "term-rewrite") ; for rewrite$-helper
+(include-book "make-test")
+
+(set-state-ok t)
+(set-induction-depth-limit 1)
+(set-slow-alist-action :break)
+(make-event (pprogn (set-warnings-as-errors t '("Use") state)
+		    (value '(value-triple nil))))
+
+; We don't need to have pseudo-termp enabled, and enabling it drastically
+; slows down certifying or loading this book.
+(local (in-theory (disable pseudo-termp)))
+ 
+(fty::defalist nat-ttmrg-alist
+  :key-type natp
+  :val-type ttmrg-p
+  :true-listp nil)  ; fast-alist's are not true-listp's
+
+(fty::defprod proto-judge-acc
+  ((next-index natp :default 0)
+   (recognizers symbol-listp :default nil)
+   (j-alist nat-ttmrg-alist-p :default nil)))
+
+(local (defsection debug-help
+  (defines show-tterm
+    (define show-ttermx ((tterm ttmrg-p) (indent stringp))
+      :measure (ttmrg-count (ttmrg-fix tterm))
+      :returns (nothing null)
+      (b* (((ttmrg tterm) (ttmrg-fix tterm))
+	   (- (cw "~s0( expr -> ~x1~%" indent (ttmrg->expr tterm)))
+	   (indent+ (acl2::implode (list* #\Space #\Space (acl2::explode indent))))
+	   (- (cw "~s0 path-cond -> ~x1~%" indent+ tterm.path-cond))
+	   (- (cw "~s0 judgements -> ~x1~%" indent+ tterm.judgements))
+	   (- (show-guts tterm.guts indent+)))
+	(cw "~s0)~%" indent)))
+
+    (define show-guts ((guts ttmrg-guts-p) (indent stringp))
+      :measure (ttmrg-guts-count (ttmrg-guts-fix guts))
+      :returns (nothing null)
+      (ttmrg-guts-case guts
+        :if
+	  (b* ((indent+ (acl2::implode (list* #\Space #\Space (acl2::explode indent))))
+	       (- (cw "~s0 condx ->~%" indent))
+	       (- (show-ttermx guts.condx indent+))
+	       (- (cw "~s0 thenx ->~%" indent))
+	       (- (show-ttermx guts.thenx indent+))
+	       (- (cw "~s0 elsex ->~%" indent))
+	       (- (show-ttermx guts.elsex indent+)))
+	    nil)
+        :fncall
+	  (b* ((indent+ (acl2::implode (list* #\Space #\Space (acl2::explode indent))))
+	       (- (cw "~s0 args -> (~%" indent))
+	       (- (show-args guts.args indent+)))
+	    (cw "~s0)~%" indent))
+        :otherwise nil))
+
+    (define show-args ((args ttmrg-list-p) (indent stringp))
+      :measure (ttmrg-list-count (ttmrg-list-fix args))
+      :returns (nothing null)
+      (b* ((args (ttmrg-list-fix args))
+	   ((unless args) nil)
+	   ((cons hd tl) args)
+	   (- (show-ttermx hd indent)))
+	(show-args tl indent))))
+
+  (define show-tterm ((tterm ttmrg-p))
+    :returns (nothing null)
+    (show-ttermx tterm ""))
+
+	
+  (define flatten-tr (x acc)
+    :returns (flat acl2::any-p)
+    (if (consp x)
+      (flatten-tr (car x) (flatten-tr (cdr x) acc))
+      (if x (cons x acc) acc))
+    ///
+    (more-returns
+      (flat :name true-listp-of-flatten-tr
+	    (implies (true-listp acc) (true-listp flat)))))
+
+  (define flatten (x)
+    :returns (flat acl2::any-p)
+    (flatten-tr x nil)
+    ///
+    (more-returns
+      (flat :name true-listp-of-flatten (true-listp flat))))
+
+  (define bad-equal (who x j-alist val)
+    :returns (v acl2::any-p)
+    (prog2$
+      (and (member 'my-equal (flatten val))
+	   (er hard? 'bad-equal "bad my-equal: (~x0 ~x1 ~x2) -> ~x3~%" who x j-alist val))
+      val)
+    ///
+    (more-returns (v :name bad-equal-is-identity (equal v val))))
+
+  (define show-j-alist-help ((a nat-ttmrg-alist-p))
+    (b* (((unless (consp a)) nil)
+	 ((cons (cons index tterm) tl) a)
+	 (- (cw "( expr -> ~x0~%" (ttmrg->expr tterm)))
+	 (- (cw "  index -> ~x0~%" index))
+	 (- (cw "  path-cond -> ~x0~%" (ttmrg->path-cond tterm)))
+	 (- (cw "  judgements -> ~x0 )~%" (ttmrg->judgements tterm))))
+      (show-j-alist-help tl)))
+
+  (define show-j-alist((j-alist nat-ttmrg-alist-p))
+    (show-j-alist-help (set::mergesort j-alist)))))
+
+(defsection path-cond
+  :short "Propagate the path-cond down an expression tree."
+  :long  "Most functions just propagate their path-cond to their arguments.
+(if cond then else) strengthens the path-cond of its then and else
+with cond and (not cond) respectively."
+
+  ; negate: simple version.
+  ;   BOZO: rather than constructing a new pseudo-term (list 'not x), I should
+  ;   at least check and simplify (not (not ...)).
+  (define negate ((x pseudo-termp))
+    :returns (not-x pseudo-termp)
+    (b* ((x (pseudo-term-fix x))
+	 (nx (list 'not x))
+	 ((unless (consp x)) nx)
+	 ((if (equal (car x) 'not)) (cadr x))
+	 ((unless (equal (car x) 'if)) nx)
+	 ((if (and (equal (caddr x) ''t) (equal (caddr x) ''nil)))
+	  (negate (cadr x)))
+	 ((if (and (equal (caddr x) ''nil) (equal (caddr x) ''t)))
+	  (cadr x)))
+      nx)
+    ///
+    (more-returns
+      (not-x :name correctness-of-negate
+	(iff (ev-smtcp not-x a)
+	     (not (ev-smtcp (pseudo-term-fix x) a)))
+	:hints(("Goal" :in-theory (enable negate))))))
+  (define parse-conjunct-helper
+      ((term pseudo-termp) (acc pseudo-term-listp))
+    :returns (conjuncts pseudo-term-listp)
+    :verify-guards nil
+    (b* ((term (pseudo-term-fix term))
+	 (acc (pseudo-term-list-fix acc))
+	 ((if (equal term ''t)) acc)
+	 ((unless (and (consp term) (consp (cdr term)) (consp (cddr term))
+		       (consp (cdddr term)) (not (cddddr term))
+		       (equal (car term) 'if)
+		       (equal (cadddr term) ''nil)))
+	  (cons term acc))
+	 (condx (cadr term))
+	 (thenx (caddr term)))
+      (parse-conjunct-helper
+       thenx
+       (parse-conjunct-helper condx acc)))
+    ///
+    (verify-guards parse-conjunct-helper)
+
+    (more-returns
+      (conjuncts :name correctness-of-parse-conjunct-helper
+	(equal (all-list<pseudo-term-ev> conjuncts a)
+	       (and (ev-smtcp (pseudo-term-fix term) a)
+		    (ev-and-list (pseudo-term-list-fix acc) a)))
+	:hints(("Goal"
+	  :in-theory (e/d (parse-conjunct-helper pseudo-term-ev)
+			  (pseudo-term-list-equiv-implies-equal-ev-and-list-1)))))))
+
+  (define parse-conjunct ((term pseudo-termp))
+    :returns pset
+    (std::mergesort (parse-conjunct-helper term nil))
+    ///
+    (more-returns
+      (pset :name pseudo-term-set-p-of-parse-conjunct
+	(pseudo-term-set-p pset))
+
+      (pset :name correctness-of-parse-conjunct
+	(iff (all<pseudo-term-ev> pset a)
+	     (ev-smtcp (pseudo-term-fix term) a)))))
+
+  (define ttmrg-list-update-path-cond ((lst ttmrg-list-p) (parent ttmrg-p))
+    :returns (new-lst ttmrg-list-p)
+    (if (consp lst)
+      (cons (ttmrg-add-path-cond-tterm (car lst) parent)
+	    (ttmrg-list-update-path-cond (cdr lst) parent))
+      nil)
+    ///
+    (defcong ttmrg-list-equiv ttmrg-list-equiv
+	     (ttmrg-list-update-path-cond lst parent) 1
+      :hints(("Goal" :induct (pairlis$ lst lst-equiv))))
+    (defcong ttmrg->path-cond-equiv ttmrg-list-equiv
+	     (ttmrg-list-update-path-cond lst parent) 2
+      :hints(("Goal" :induct (len lst))))
+    (more-returns
+      (new-lst :name ttmrg-list->expr-list-equiv-of-ttmrg-list-update-path-cond
+	(ttmrg-list->expr-list-equiv new-lst lst))
+
+      (new-lst :name ttmrg-list-correct-p-of-ttmrg-list-update-path-cond
+	(implies (ttmrg-list-correct-p lst a)
+		 (ttmrg-list-correct-p new-lst a)))
+
+      (new-lst :name args->path-cond-ev-of-ttmrg-list-update-path-cond
+	(implies (and (ttmrg->path-cond-ev parent a)
+		      (args->path-cond-ev lst a))
+		 (args->path-cond-ev new-lst a)))))
+
+  (define ttmrg-update-path-cond-children ((tterm ttmrg-p))
+    :returns (new-tt ttmrg-p)
+    (case (ttmrg->kind tterm)
+      (:var (ttmrg-fix tterm))
+      (:quote (ttmrg-fix tterm))
+      (:if
+	(b* ((condx (ttmrg->condx tterm))
+	     (thenx (ttmrg->thenx tterm))
+	     (elsex (ttmrg->elsex tterm))
+	     (cond-expr  (ttmrg->expr condx)))
+	  (change-ttmrg
+	    tterm
+	    :guts
+	    (change-ttmrg-guts-if
+	      (ttmrg->guts tterm)
+	      :condx (ttmrg-add-path-cond-tterm condx tterm)
+	      :thenx (ttmrg-add-path-cond-set
+		       (ttmrg-add-path-cond-tterm thenx tterm)
+		       (parse-conjunct cond-expr))
+	      :elsex (ttmrg-add-path-cond-set
+		       (ttmrg-add-path-cond-tterm elsex tterm)
+		       (parse-conjunct (negate cond-expr)))))))
+      (:fncall
+	(b* ((new-args (ttmrg-list-update-path-cond (ttmrg->args tterm) tterm))
+	     (new-guts (make-ttmrg-guts-fncall
+			 :f (ttmrg->f tterm)
+			 :args new-args)))
+	  (make-ttmrg :path-cond (ttmrg->path-cond tterm)
+		      :judgements (ttmrg->judgements tterm)
+		      :smt-judgements (ttmrg->smt-judgements tterm)
+		      :guts new-guts))))
+    ///
+    (defcong ttmrg-equiv ttmrg-equiv (ttmrg-update-path-cond-children tterm) 1)
+    (more-returns
+      (new-tt :name ttmrg->path-cond-of-ttmrg-update-path-cond-children
+	(ttmrg->path-cond-equiv new-tt tterm))
+
+      (new-tt :name ttmrg->judgements-of-ttmrg-update-path-cond-children
+	      (ttmrg->judgements-equiv new-tt tterm))
+
+      (new-tt :name ttmrg->smt-judgements-of-ttmrg-update-path-cond-children
+	      (ttmrg->smt-judgements-equiv new-tt tterm))
+
+      (new-tt :name ttmrg->kind-of-ttmrg-update-path-cond-children
+	(ttmrg->kind-equiv new-tt tterm))))
+
+  (local (defrule ttmrg-equiv-of-var-or-quote
+    (implies
+      (or (equal (ttmrg->kind tterm) :var)
+	  (equal (ttmrg->kind tterm) :quote))
+      (ttmrg-equiv (ttmrg-update-path-cond-children tterm)
+		   tterm))
+    :in-theory (enable ttmrg-update-path-cond-children)))
+
+  (local (defrule lemma-if-details
+    (let* ((condx (ttmrg->condx tterm))
+	   (thenx (ttmrg->thenx tterm))
+	   (elsex (ttmrg->elsex tterm))
+	   (cond-expr  (ttmrg->expr condx))
+	   (new-tt (ttmrg-update-path-cond-children tterm))
+	   (new-condx (ttmrg-add-path-cond-tterm condx tterm))
+	   (new-thenx (ttmrg-add-path-cond-set
+			(ttmrg-add-path-cond-tterm thenx tterm)
+			(parse-conjunct cond-expr)))
+	   (new-elsex (ttmrg-add-path-cond-set
+			(ttmrg-add-path-cond-tterm elsex tterm)
+			(parse-conjunct (negate cond-expr)))))
+      (implies (equal (ttmrg->kind tterm) :if)
+	       (and (ttmrg-equiv (ttmrg->condx new-tt) new-condx)
+		    (ttmrg-equiv (ttmrg->thenx new-tt) new-thenx)
+		    (ttmrg-equiv (ttmrg->elsex new-tt) new-elsex))))
+    :in-theory (enable ttmrg-update-path-cond-children)))
+
+  (local (defrule lemma-fncall-details
+    (implies (equal (ttmrg->kind tterm) :fncall)
+      (let* ((new-tt (ttmrg-update-path-cond-children tterm))
+	     (args (ttmrg->args tterm))
+	     (new-args (ttmrg->args new-tt)))
+	(ttmrg-list-equiv new-args (ttmrg-list-update-path-cond args tterm))))
+    :in-theory (enable ttmrg-update-path-cond-children)))
+
+  (local (defrule ttmrg->judgements-and-expr-of-ttmrg-update-path-cond-children
+    (let ((new-tt (ttmrg-update-path-cond-children tterm)))
+      (and (ttmrg->judgements-and-expr-equiv new-tt tterm)
+	   (ttmrg->smt-judgements-and-expr-equiv new-tt tterm)))
+    :in-theory (enable ttmrg->judgements-and-expr-equiv
+		       ttmrg->smt-judgements-and-expr-equiv)
+    :prep-lemmas (
+      (defrule lemma-fncall-f
+	(let ((new-tt (ttmrg-update-path-cond-children tterm)))
+	  (implies (equal (ttmrg->kind tterm) :fncall)
+		   (ttmrg->f-equiv new-tt tterm)))
+	:in-theory (enable ttmrg-update-path-cond-children
+			   ttmrg->f ttmrg->f-equiv))
+      (defrule lemma-equal
+	(let ((new-tt (ttmrg-update-path-cond-children tterm)))
+	  (equal (ttmrg->expr new-tt) (ttmrg->expr tterm)))
+	:use((:instance
+	       ttmrg->expr (tterm (ttmrg-update-path-cond-children tterm)))
+	     (:instance ttmrg->expr))))))
+
+  (defrule ttmrg->expr-of-ttmrg-update-path-cond-children
+    (let ((new-tt (ttmrg-update-path-cond-children tterm)))
+      (ttmrg->expr-equiv new-tt tterm)))
+
+  (defrule ttmrg-correct-p-of-ttmrg-update-path-cond-children
+    (let ((new-tt (ttmrg-update-path-cond-children tterm)))
+      (implies (ttmrg-correct-p tterm a)
+	       (ttmrg-correct-p new-tt a)))
+    :expand ((ttmrg-correct-p (ttmrg-update-path-cond-children tterm) a)))
+
+  (define ttmrg-upcc-ignore-options-and-state
+      ((tterm ttmrg-p) (opts acl2::any-p) (state state-p))
+    :ignore-ok t
+    (ttmrg-update-path-cond-children tterm))
+
+  (in-theory (enable ttmrg-upcc-ignore-options-and-state))
+  (ttmrg-propagate path-cond :pre ttmrg-upcc-ignore-options-and-state)
+  (in-theory (disable ttmrg-upcc-ignore-options-and-state)))
+
+(defsection proto-judgements
+  :short "add judgements to each subterm of a ttmrg"
+  :long  "Add judgements to a ttmrg of the form
+    (my-equal (hide (cdr (cons expr-index (type-p x)))) (type-p x))
+for each type-recognizer, type-p, known to smtlink.  We'll use rewrite$ to simplify
+the ttmrg-correct-expr generated from these judgements.  This allows us to connect
+the hidden (type-p x) with the unhidden, and thus rewritten (type-p x).  rewrite$
+can change the structure of the term.  We use expr-index to match to the correct
+instance of a sub-expression."
+; Implementation note 1: This seems like a nice task for the ttmrg-propagate macro
+;   from the ttmrg-change3 book.  But, it doesn't provide a way to thread the counter
+;   through the tree walk.  I could modify the macro (or write a new one) that return
+;   (mv new-counter new-ttmrg-node), but that will add clutter of either having two
+;   version of the macro, or forcing the smtlink developer to provide updating functions
+;   that return an mv, even when they don't need it.  I could store counter in a table
+;   in state.  That should work because we are planning on calling rewrite$ from a
+;   computed-hint.  However, if we wanted similar functionality in a clause processor,
+;   we can't modify state.  So, I'm writing a tree-walker just for this use.
+
+;   Implementation note 2: Checking every subterm against every type recognizer may
+;   introduce scaling issues if smtlink is used on big clauses with a large set of
+;   possible types.  We could probably check the returns theorems for the top-level
+;   function of each subterm to get a set of possible types.  I'm not sure how we
+;   find these rules for highly-overloaded functions such as car and cdr.
+;
+;   Implementaion note 3: Because the judgements we add are trivial tautologies,
+;   adding these judgements should preserve ttmrg-correct-p.  I haven't included
+;   a proof because we have to verify the result of rewrite$ at run-time anyway.
+
+  (define my-equal ((x acl2::any-p) (y acl2::any-p))
+    :returns (ok booleanp)
+    (equal x y))
+
+  (define proto-judge-help ((recognizers symbol-listp) (expr-index natp))
+    :returns (judges judge-set-p
+		     :hints(("Goal" :in-theory (enable judge-p))))
+    :measure (len recognizers)
+    (b* (((if (endp recognizers)) nil)
+	 ((cons rec tl) (symbol-list-fix recognizers)))
+       (set::insert
+	 `(my-equal (hide (cdr (cons ,(kwote expr-index) (,rec x))))
+		    (bool-fix$inline (,rec x)))
+	  (proto-judge-help tl expr-index))))
+
+  (defines proto-judgements
+    :verify-guards nil
+    (define proto-judgements-term ((tterm ttmrg-p) (acc proto-judge-acc-p))
+      :returns (mv (new-tt ttmrg-p) (new-acc proto-judge-acc-p))
+      :measure (ttmrg-count (ttmrg-fix tterm))
+      :flag term
+      (b* (((mv guts-x acc-x)
+	    (proto-judgements-guts (ttmrg->guts tterm) acc))
+	   ((proto-judge-acc acc-x) acc-x)
+	   (new-tt
+	    (change-ttmrg tterm
+	      :guts guts-x
+	      :judgements
+		(proto-judge-help acc-x.recognizers acc-x.next-index)))
+	   (new-acc
+	     (change-proto-judge-acc acc-x
+	       :next-index (1+ acc-x.next-index)
+	       :j-alist (hons-acons acc-x.next-index new-tt acc-x.j-alist))))
+	(mv new-tt new-acc)))
+		
+    (define proto-judgements-guts
+	((guts ttmrg-guts-p)  (acc proto-judge-acc-p))
+      :returns (mv (new-guts ttmrg-guts-p) (new-acc proto-judge-acc-p))
+      :measure (ttmrg-guts-count (ttmrg-guts-fix guts))
+      :flag guts
+      (b* ((guts (ttmrg-guts-fix guts))
+	   (acc0 (proto-judge-acc-fix acc)))
+	(ttmrg-guts-case guts
+	   :var (mv guts acc0)
+	   :quote (mv guts acc0)
+	   :if 
+	     (b* (((mv new-condx acc1)
+		   (proto-judgements-term guts.condx acc0))
+		  ((mv new-thenx acc2)
+		   (proto-judgements-term guts.thenx acc1))
+		  ((mv new-elsex acc3)
+		   (proto-judgements-term guts.elsex acc2)))
+	      (mv (change-ttmrg-guts-if guts
+		    :condx new-condx :thenx new-thenx :elsex new-elsex)
+		  acc3))
+	   :fncall 
+	     (b* (((mv new-args acc1)
+		   (proto-judgements-list guts.args acc0)))
+	       (mv (change-ttmrg-guts-fncall guts :args new-args)
+		   acc1)))))
+
+    (define proto-judgements-list
+	((ttlst ttmrg-list-p) (acc proto-judge-acc-p))
+      :returns (mv (new-ttlst ttmrg-list-p) (new-acc proto-judge-acc-p))
+      :measure (ttmrg-list-count (ttmrg-list-fix ttlst))
+      :flag list
+      (b* ((ttlst (ttmrg-list-fix ttlst))
+	   ((proto-judge-acc acc0) (proto-judge-acc-fix acc))
+	   ((unless (consp ttlst)) (mv nil acc0))
+	   ((cons hd tl) ttlst)
+	   ((mv new-hd acc1) (proto-judgements-term hd acc0))
+	   ((mv new-tl acc2) (proto-judgements-list tl acc1)))
+	(mv (cons new-hd new-tl) acc2)))
+    ///
+    (verify-guards proto-judgements-term))
+
+  ; The case-match in parse-my-equal below nicely (imho) expresses the pattern
+  ;   we want to handle for (my-equal ...) expressions returned by rewrite$.
+  ;   It also causes prolific case splitting.  To manage this, we quarantine
+  ;   the case-match in parse-my-equal and process the results of the
+  ;   case-match in parese-my-equal-help.
+  (define parse-my-equal-help ((js nat-ttmrg-alist-p) (i natp) (j judge-p))
+    :returns (new-js nat-ttmrg-alist-p)
+    :verify-guards nil
+    (b* ((js (nat-ttmrg-alist-fix js))
+	 (i (nfix i))
+	 (j (judge-fix j))
+	 (a (hons-get i js))
+	 ((unless a)
+	  (er acl2::hard? 'parse-my-equal
+	      "Smtlink internal error: bad expr-index, ~x0~%" i))
+	 ((ttmrg tt0) (cdr a))
+	 (tt1 (if (and (not (set::emptyp tt0.judgements))
+		       (consp (set::head tt0.judgements))
+		       (equal (car (set::head tt0.judgements)) 'my-equal))
+		(change-ttmrg tt0 :judgements nil)
+		tt0)))
+      (hons-acons i (ttmrg-add-judge-set tt1 (list j)) js))
+    ///
+    (local (defrule guard-lemma
+      (implies (judge-p j) (judge-set-p (list j)))
+      :enable judge-set-p))
+    (verify-guards parse-my-equal-help))
+
+  (define parse-my-equal ((js nat-ttmrg-alist-p) (x pseudo-termp))
+    :returns (new-js nat-ttmrg-alist-p)
+    :verify-guards nil
+    (let ((js (nat-ttmrg-alist-fix js)))
+      (case-match x
+	(('my-equal ('hide ('cdr ('cons ('quote expr-index) (type-recognizer &)))) ''t)
+	 (if (and (natp expr-index) (symbolp type-recognizer))
+	   (parse-my-equal-help js expr-index `(,type-recognizer x))
+	   js))
+	(& js)))
+    ///
+    (local (defrule guard-lemma
+      (implies (symbolp type-recognizer) (judge-p `(,type-recognizer x)))
+      :enable judge-p))
+    (verify-guards parse-my-equal))
+
+
+  (define delete-empty-judgements ((js nat-ttmrg-alist-p) (keys nat-listp))
+    :measure (len (acl2::nat-list-fix keys))
+    :returns (new-js nat-ttmrg-alist-p)
+    (b* ((js (nat-ttmrg-alist-fix js))
+	 (keys (acl2::nat-list-fix keys))
+	 ((unless keys) js)
+	 ((cons hd tl) keys)
+	 (a (hons-get hd js))
+	 ((unless (consp a)) js) ; shouldn't happen
+	 ((ttmrg tt) (cdr a))
+	 (js2 (if (and (consp tt.judgements)
+		       (consp (car tt.judgements))
+		       (equal (caar tt.judgements) 'my-equal))
+		(hons-acons hd (change-ttmrg tt :judgements nil) js)
+		js)))
+      (delete-empty-judgements js2 tl)))
+
+  (define parse-judgements-help ((js nat-ttmrg-alist-p) (x pseudo-termp))
+    :returns (new-js nat-ttmrg-alist-p)
+    :verify-guards nil
+    (b* ((js (nat-ttmrg-alist-fix js))
+	 (x (pseudo-term-fix x))
+	 ((unless (equal (acl2::pseudo-term-kind x) :fncall)) js)
+	 ((if (equal (acl2::pseudo-term-fncall->fn x) 'my-equal))
+	  (parse-my-equal js x))
+	 ((unless (equal (acl2::pseudo-term-fncall->fn x) 'if)) js)
+	 (args (acl2::pseudo-term-fncall->args x))
+	 ((unless (and (consp args)
+		       (consp (cdr args))
+		       (consp (cddr args))
+		       (null (cdddr args))))
+	  js)
+	 ((list condx thenx elsex) args))
+      (parse-judgements-help
+	(parse-judgements-help
+	  (parse-judgements-help js condx) thenx) elsex))
+    ///
+    (verify-guards parse-judgements-help))
+
+  (define j-alist-keys ((js nat-ttmrg-alist-p))
+    :returns (keys nat-listp)
+    :measure (len (nat-ttmrg-alist-fix js))
+    :short "Like strip-cars without the guard of alistp."
+    :long "Alistp implies true-listp, but fast-alists don't satisfy alistp!"
+    (b* ((js (nat-ttmrg-alist-fix js))
+	 ((unless (consp js)) nil)
+	 ((cons hd tl) js))
+      (cons (car hd) (j-alist-keys tl))))
+
+  (define parse-judgements ((js nat-ttmrg-alist-p) (x pseudo-termp))
+    :returns (new-js nat-ttmrg-alist-p)
+    (b* ((js1 (parse-judgements-help js x))
+	 (keys (j-alist-keys js1)))
+    (fast-alist-clean
+      (delete-empty-judgements (parse-judgements-help js1 x) keys)))))
+
+(defsection merge-judgements
+  :short "Annotate a term with the type-judgements determined by rewrite$."
+  :long  "Emperically, applying rewrite$ to the  ttmrg-correct-expr of a term
+returns an if-then-else tree where the conditions are the path-conditions of
+the term.  If an if-condition, then-expression, or else-expression is an
+application of my-equal, we check to see if the unhidden version of the
+type-recognizer call rewrote to 't.  If so, we add that type-judgement
+to the term."
+
+  (define merge-judgements-fetch ((tt-proto ttmrg-p) (j-alist nat-ttmrg-alist-p))
+    :returns (new-tt ttmrg-p)
+    (b* (((ttmrg tt-proto) (ttmrg-fix tt-proto))
+	 (j-alist (nat-ttmrg-alist-fix j-alist))
+	 (j1
+	   (if (set::emptyp tt-proto.judgements)
+	     'missing-judgements
+	     (set::head tt-proto.judgements)))
+	 (tt3 (case-match j1
+		(('my-equal ('hide ('cdr ('cons ('quote expr-index) &))) &)
+		 (b* (((unless (natp expr-index))
+		       (er hard? 'merge-judgements-fetch
+			   "Smtlink, internal error: expr-index is not a natp -- ~x0"
+			   expr-index))
+		      (a (hons-get expr-index j-alist))
+		      ((unless a)
+		       (er hard? 'merge-judgements-fetch
+			   "Smtlink, internal error: expr-index not found in j-alist -- expr-index = ~x0"
+			   expr-index))
+		      ((ttmrg tt1) (cdr a)))
+		   tt1))
+		('missing-judgements
+		 (er hard? 'merge-judgements-fetch
+		     "Smtlink, internal error: tt-proto has no judgements"))
+		(& (er hard? 'merge-judgements-fetch
+		       "tt-proto judgements aren't my-equal tests"))))
+	 )
+	(if tt3 tt3 tt-proto)))
+
+
+  (defines merge-judgements
+    :verify-guards nil
+    (define merge-judgements-term ((tt-proto ttmrg-p)
+				  (j-alist nat-ttmrg-alist-p))
+      :measure (ttmrg-count (ttmrg-fix tt-proto))
+      :returns (new-tt ttmrg-p)
+      (change-ttmrg (merge-judgements-fetch tt-proto j-alist)
+	:guts (merge-judgements-guts (ttmrg->guts tt-proto) j-alist)))
+
+    (define merge-judgements-guts ((guts ttmrg-guts-p)
+				   (j-alist nat-ttmrg-alist-p))
+      :measure (ttmrg-guts-count (ttmrg-guts-fix guts))
+      :returns (new-guts ttmrg-guts-p)
+      (b* ((guts (ttmrg-guts-fix guts))
+	   (j-alist (nat-ttmrg-alist-fix j-alist)))
+	(ttmrg-guts-case guts
+	  :var guts
+	  :quote guts
+	  :if
+	    (change-ttmrg-guts-if guts
+	      :condx (merge-judgements-term guts.condx j-alist)
+	      :thenx (merge-judgements-term guts.thenx j-alist)
+	      :elsex (merge-judgements-term guts.elsex j-alist))
+	  :fncall
+	    (change-ttmrg-guts-fncall guts
+	      :args (merge-judgements-args guts.args j-alist))))
+    )
+	    
+    (define merge-judgements-args ((args-proto ttmrg-list-p)
+				   (j-alist nat-ttmrg-alist-p))
+      :measure (ttmrg-list-count (ttmrg-list-fix args-proto))
+      :returns (new-ttlst ttmrg-list-p)
+      (b* ((args-proto (ttmrg-list-fix args-proto))
+	   ((unless args-proto) nil)
+	   ((cons hd tl) args-proto))
+	(cons (merge-judgements-term hd j-alist)
+	      (merge-judgements-args tl j-alist))))
+    ///
+    (verify-guards merge-judgements-term)))
+
+(define type-inference-rw ((expr pseudo-termp)
+			   (recognizers symbol-listp)
+			   (state state-p))
+  :mode :program
+  (b* ((expr (pseudo-term-fix expr))
+       (recognizers (symbol-list-fix recognizers))
+       ((proto-judge-acc acc) (make-proto-judge-acc :recognizers recognizers))
+       (tt1 (ttmrg-propagate-path-cond-term
+	      (make-ttmrg-trivial expr) nil state)))
+    (with-fast-alist acc.j-alist
+      (b* (((mv tt2 acc2)
+	    (proto-judgements-term tt1 acc))
+	   ((unless (termp (ttmrg-correct-expr tt2) (w state)))
+	    (er soft 'type-inference-rw "(termp (ttmrg-correct-expr xpre) (w state)) -> nil~%"))
+	   (cx2 (acl2::beta-reduce-pseudo-termp (ttmrg-correct-expr tt2)))
+	   ((mv erp cx2-rw state)
+	    (rewrite$-helper cx2 nil nil state))
+	   ((if erp)
+	    (prog2$
+	      (cw "rewrite$-helper failed: erp=~x0, cx2-rw=~x1~%" erp cx2-rw)
+	      (mv erp cx2-rw state)))
+	   (- (cw "cx2-rw = ~x0~%" cx2-rw))
+	   (j (fast-alist-clean (parse-judgements (proto-judge-acc->j-alist acc2) cx2-rw)))
+	   (tt3 (merge-judgements-term tt2 j)))
+	(value tt3)))))
+
+(define smt-recognizers ((datatypes smt-datatype-list-p))
+  :returns (recognizers symbol-listp)
+  :measure (len (smt-datatype-list-fix datatypes))
+  (b* ((datatypes (smt-datatype-list-fix datatypes))
+       ((unless datatypes) nil)
+       ((cons hd tl) datatypes))
+    (cons (smt-function->name (smt-datatype->recognizer hd))
+	  (smt-recognizers tl))))
+
+(define smt-type-judge-bottom-up-hint (cl kwd-alist state)
+    :guard-debug t
+    :parents (smt-computed-hints)
+    :short "@('smt::smt-type-judge-bottom-up-hint') WRITE SOMETHING."
+    :mode :program
+    (b* (((unless (and (pseudo-term-listp cl)
+                       (consp kwd-alist)
+                       (consp (cdr kwd-alist))
+                       (consp (cadr kwd-alist))
+                       (= (len (cadr kwd-alist))
+                          4)
+                       (state-p state)))
+          (prog2$ (cw "smt-type-judge-bottom-up-hint: preconditions not met: ~x0~%"
+		      (if (pseudo-term-listp cl)
+                         (if (consp kwd-alist)
+                           (if (consp (cdr kwd-alist))
+			     (if (consp (cadr kwd-alist))
+			       (if (= (len (cadr kwd-alist)) 4)
+				 (if (state-p state)
+				   "all preconditions satisfied?!"
+				   "(not (state-p state))")
+				 "(not (= (len (cadr kwd-alist)) 4))")
+			       "(not (consp (cadr kwd-alist)))")
+			     "(not (consp (cdr kwd-alist)))")
+			   "(not (consp kwd-alist))")
+			 "(not (psuedo-term-listp cl))"))
+                  (value nil)))
+         ((list* cp-kwd (list next-cp & q-smt-hint &) kwd-alist-tail) kwd-alist)
+         ((unless (equal cp-kwd :clause-processor))
+          (prog2$ (cw "smt-term-rewrite-hint: missing clause processor in kwd-alist: ~x0~%"
+                      kwd-alist)
+                  (value nil)))
+         ((unless (and (quotep q-smt-hint)
+                       (smtlink-hint-p (unquote q-smt-hint))))
+          (prog2$ (cw "not quoted smtlink-hint-p: ~x0~%" q-smt-hint)
+                  (value nil)))
+         (smt-hint (unquote q-smt-hint))
+         (recognizers (smt-recognizers (smtlink-hint->datatypes smt-hint)))
+         (goal (disjoin cl))
+	 ((mv fail tterm state) (type-inference-rw goal recognizers state))
+         ((if fail) (value nil)))
+      (prog2$ (cw "smt-term-rewrite-hint~%  goal: ~x0~%  tterm: ~x1~%"
+                  goal
+                  tterm)
+              (value `(:computed-hint-replacement ((smt-computed-hint clause))
+                       :clause-processor (,next-cp clause ',(cons smt-hint tterm) state)
+                       ,@kwd-alist-tail)))))
+
+(define type-judge-bottom-up-cp ((cl pseudo-term-listp) (hint t) state)
+    (b* (((unless (pseudo-term-listp cl)) (mv t nil state))
+         (goal (disjoin cl))
+         ((unless (consp hint)) (mv t nil state))
+         ((cons smt-hint tterm) hint)
+         ((unless (smtlink-hint-p smt-hint)) (mv t nil state))
+         ((unless (ttmrg-p tterm)) (mv t nil state))
+	 ((unless (equal (ttmrg->expr tterm) goal))
+	  (prog2$
+	    (cw "type-judge-bottom-up-cp: tterm.expr doesn't match goal.~%  goal: ~x0~%  tterm.expr: ~x1~%"
+		goal (ttmrg->expr tterm))
+	    (mv t nil state)))
+	 (next-cp (cdr (assoc-equal 'type-judge-bottom-up *SMT-architecture*)))
+	 ((if (null next-cp)) (mv t nil state))
+	 (new-cl (ttmrg-clause tterm))
+	 (the-hint `(:clause-processor (,next-cp clause ',smt-hint state)))
+	 (hinted-goal `((hint-please ',the-hint) ,new-cl))
+	 ;; Side condition
+	 (side-condition (ttmrg-correct-expr tterm))
+	 ; might add a theory hint based on the rules used by rewrite$, or
+	 ;   allow hints from the (advanced?) user.
+	 )
+      (value (list (list side-condition) hinted-goal))))
+
+(defrule correctness-of-type-judge-bottom-up-cp
+    (implies (and (pseudo-term-listp cl)
+                  (alistp a)
+                  (ev-smtcp
+                    (conjoin-clauses
+                      (acl2::clauses-result
+                        (type-judge-bottom-up-cp cl hint state)))
+                    a))
+             (ev-smtcp (disjoin cl) a))
+    :do-not-induct t
+    :expand (type-judge-bottom-up-cp cl hint state)
+    :in-theory (disable ev-smtcp-of-disjoin)
+    :rule-classes :clause-processor)
+
+
+(local (defsection examples
+  (fty::defalist nat-sym-alist
+    :key-type natp
+    :val-type symbolp
+    :true-listp t)
+
+  (define xpr ()
+    :returns (x pseudo-termp)
+    '(if (natp x)
+       (if (integerp y)
+	 (natp (binary-+ x (binary-* y y)))
+       't)
+     't))
+
+  (define xpr2 ()
+    :returns (x pseudo-termp)
+    '(if (natp x)
+       (if (not (integerp y))
+	  (natp (binary-+ x (binary-* y y)))
+       't)
+     't))
+
+  (define expr-pre ((expr pseudo-termp) (state state-p))
+    (b* (((proto-judge-acc acc)
+	  (make-proto-judge-acc
+	    :recognizers '(booleanp integerp natp nat-sym-alist-p)))
+	 (tt1 (ttmrg-propagate-path-cond-term
+		(make-ttmrg-trivial expr) nil state)))
+      (with-fast-alist acc.j-alist
+	(proto-judgements-term tt1 acc))))
+
+  (define rec()
+    :returns (recognizers symbol-listp)
+    '(booleanp integerp natp nat-sym-alist-p))
+
+  (define rw-test-fn ((expr pseudo-termp))
+    `(b* ((recognizers '(booleanp integerp natp nat-sym-alist-p))
+	  ((mv erp tterm state) (type-inference-rw ,expr recognizers state))
+	  ((if erp)
+	   (prog2$ (cw "type-inference-rw failed~%")
+		   (mv erp tterm state)))
+	  ((unless (ttmrg-p tterm))
+	   (er soft 'rw-test
+	       "type-inference-rw should return (mv nil x state) where (ttmrg-p x))~%  but x is not a ttmrg-p~%  x = ~x0~%"
+	       tterm))
+	  (- (cw "tterm = ~%"))
+	  (- (show-ttermx tterm "  ")))
+       (mv nil 'ok state))
+    ///
+    (defmacro rw-test (expr)
+      (rw-test-fn expr)))
+
+  ; for an example, try
+  ; (rw-test (xpr))
+
+(define smt-type-judge-bottom-up-demo (state)
+  :mode :program
+  (b* (((mv fail x state)
+	(smt-type-judge-bottom-up-hint
+	  (list (xpr))
+	  (list :clause-processor
+		(list 'type-judge-top-down
+		      'ignore-me
+		      (kwote
+			(make-smtlink-hint
+			  :datatypes
+			  (list (make-smt-datatype-basic :recognizer (make-smt-function :name 'booleanp))
+				(make-smt-datatype-basic :recognizer (make-smt-function :name 'integerp))
+				(make-smt-datatype-basic :recognizer (make-smt-function :name 'natp))
+				(make-smt-datatype-basic :recognizer (make-smt-function :name 'nat-sym-alist-p)))))
+		      'ignore-me))
+	  state))
+       ((if fail)
+	(mv fail (cw "smt-type-judge-bottom-up-hint failed~%") state))
+       (- (cw "x  = `(~x0 ~x1 ~x2~%      (~x3 ~x4 ',(cons smt-hint tterm) ~x5)~%      ...)~%"
+	      (car x) (cadr x) (caddr x) (car (cadddr x)) (cadr (cadddr x)) (cadddr (cadddr x))))
+       (- (cw "smt-hint = ~x0~%" (car (unquote (caddr (cadddr x))))))
+       (- (cw "tterm =~%"))
+       (- (show-ttermx (cdr (unquote (caddr (cadddr x)))) "  ")))
+    (value :invisible)))))
